extraction/theories/ExtractionCorrectness.v
@@ -1,1 +1,148 @@
+From ConCert.Extraction Require Import Aux.
+From ConCert.Extraction Require Import ClosedAux.
+From ConCert.Extraction Require Import Erasure.
 From ConCert.Extraction Require Import Extraction.
+From ConCert.Extraction Require Import Optimize.
+From ConCert.Extraction Require Import OptimizeCorrectness.
+From ConCert.Extraction Require Import ResultMonad.
+From ConCert.Extraction Require Import WcbvEvalType.
+From Coq Require Import List.
+From Coq Require Import String.
+From Equations Require Import Equations.
+From MetaCoq.Erasure Require Import ErasureCorrectness.
+From MetaCoq.Erasure Require Import ErasureFunction.
+From MetaCoq.Erasure Require Import EWcbvEval.
+From MetaCoq.Erasure Require Import Extract.
+From MetaCoq.Erasure Require Import Prelim.
+From MetaCoq.PCUIC Require Import PCUICAstUtils.
+From MetaCoq.PCUIC Require Import PCUICSafeLemmata.
+From MetaCoq.PCUIC Require Import PCUICTyping.
+From MetaCoq.PCUIC Require PCUICWcbvEval.
+From MetaCoq.Template Require Import BasicAst.
+From MetaCoq.Template Require Import utils.
+
+Open Scope string.
+
+Import ListNotations.
+
+Module P := PCUICAst.
+Module E := EAst.
+
+Notation "Σ 'p⊢' s ▷ t" := (PCUICWcbvEval.eval Σ s t) (at level 50, s, t at next level) : type_scope.
+Notation "Σ 'e⊢' s ▷ t" := (EWcbvEval.eval Σ s t) (at level 50, s, t at next level) : type_scope.
+
+Definition Pis_constant (decl : P.global_decl) : bool :=
+  match decl with
+  | P.ConstantDecl _ => true
+  | _ => false
+  end.
+
+Definition Ponly_constants (Σ : P.global_env) : P.global_env :=
+  filter (Pis_constant ∘ snd) Σ.
+
+Lemma Pdeclared_constant_only_constants Σ kn decl :
+  declared_constant Σ kn decl ->
+  declared_constant (Ponly_constants Σ) kn decl.
+Proof.
+  unfold declared_constant.
+  intros lookup_decl.
+  induction Σ; [easy|].
+  destruct a as (kn' & decl').
+  cbn in *.
+  destruct (Pis_constant decl') eqn:isconst.
+  - cbn in *.
+    unfold eq_kername in *.
+    destruct (kername_eq_dec _ _) as [<-|?]; easy.
+  - apply IHΣ.
+    unfold eq_kername in *.
+    destruct (kername_eq_dec _ _).
+    + inversion lookup_decl; subst; easy.
+    + auto.
+Qed.
+
+Lemma Peval_only_constants Σ s t :
+  Σ p⊢ s ▷ t ->
+  Ponly_constants Σ p⊢ s ▷ t.
+Proof.
+  induction 1; eauto using PCUICWcbvEval.eval, Pdeclared_constant_only_constants.
+Qed.
+
+Lemma eval_const_construct_expanded Σ kn ind c im cm :
+  trans_env Σ e⊢ E.tConst kn ▷ E.tConstruct ind c ->
+  valid_masks_env im cm Σ ->
+  is_expanded im cm (E.tConst kn).
+Proof.
+  intros ev valid.
+  depelim ev.
+  unfold valid_masks_env in valid.
+  apply forallb_Forall in valid.
+  apply declared_constant_trans in isdecl as (? & ? & nth).
+  eapply nth_error_forall in nth; [|eassumption].
+  cbn in *.
+  rewrite H in nth.
+  propify.
+  destruct nth as (valid_mask_body & _).
+  clear -ev valid_mask_body.
+  apply valid_dearg_mask_spec in valid_mask_body as (Γ & inner & <- & <-).
+  induction #|Γ| as [|Γlen IH] eqn:eq in Γ, inner, ev |- *.
+  - now destruct Γ.
+  - destruct Γ as [|[na [body|]] Γ]; cbn in *.
+    + easy.
+    + depelim ev.
+      refold.
+      rewrite subst_it_mkLambda_or_LetIn in ev2.
+      erewrite <- vasses_subst_context.
+      eapply IH; [eassumption|].
+      now rewrite length_subst_context.
+    + depelim ev.
+Qed.
+
+Lemma extract_correct (Σ : P.global_env_ext) kn ui ind c ui' (wfΣ : wf_ext Σ) exΣ :
+  axiom_free Σ ->
+  welltyped Σ [] (P.tConst kn ui) ->
+  Σ p⊢ P.tConst kn ui ▷ P.tConstruct ind c ui' ->
+  (isErasable Σ [] (P.tConstruct ind c ui') -> False) ->
+  extract_pcuic_env
+    (pcuic_params check_masks_args)
+    Σ (wf_ext_wf_squash wfΣ) [kn] (fun _ => false) = Ok exΣ ->
+  trans_env exΣ e⊢ E.tConst kn ▷ E.tConstruct ind c.
+Proof.
+  intros ax [T wt] ev not_erasable ex.
+  cbn in *.
+  destruct validate_erases eqn:validate; cbn in *; [|congruence].
+  destruct erase_global_decls_deps_recursive as [Σex|] eqn:er; cbn in *; [|congruence].
+  destruct env_closed eqn:closed; cbn in *; [|congruence].
+  destruct analyze_env eqn:an; cbn in *.
+  destruct is_expanded_env eqn:isexp; cbn in *; [|congruence].
+  destruct valid_masks_env eqn:valid; cbn in *; [|congruence].
+  inversion_clear ex.
+  rewrite trans_env_debox_env_types.
+
+  assert (exists Σer,
+             (erases_global Σ Σer) /\
+             (forall kn decl, In (kn, decl) (trans_env Σex) -> In (kn, decl) Σer))
+    as (Σer & erΣer & same_consts) by admit.
+  eapply erases_correct in erΣer as ever.
+  5: exact ev.
+  3: exact wt.
+  3: constructor.
+  2: now constructor.
+  destruct ever as (? & er' & ev').
+  depelim er'; [|easy].
+  { exfalso.
+    eapply subject_reduction_eval in ev; eauto.
+
+  assert (exists v', Σ;;; [] |- P.tConst kn ui ⇝ℇ v' /\ trans_env Σex e⊢ E.tConst kn ▷ v').
+  { eapply erases_correct.
+    - now constructor.
+    - easy.
+    - constructor.
+    - a
+  trans_env Σex e⊢ E.tConst kn ▷ E.tConstruct ind c).
+  { eapply erases_correct.
+  apply Peval_only_constants in ev.
+Lemma validate_erases_erases_global Σ wfΣ :
+  validate_erases erase_func Σ wfΣ ->
+  erase_global_decls_deps_recursive erase_func Σ wfΣ
+  erases_global (Ponly_constants Σ) (trans_env Σex)
+  Admitted.
