extraction/theories/MetaCoqErasureCorrectnessStrong.v
@@ -1,0 +1,1284 @@
+(* This file copies the erasure correctness proof from MetaCoq and strengthens it
+   for our use where where we do not erase full environments but rather only dependencies. *)
+
+From Coq Require Import Bool String List Program.Basics Program.Tactics ZArith.
+From MetaCoq.Template Require Import config utils monad_utils.
+From MetaCoq.Erasure Require Import ELiftSubst ETyping EWcbvEval Extract Prelim
+     ESubstitution EInversion EArities.
+From MetaCoq.PCUIC Require Import PCUICTyping PCUICAst PCUICAstUtils
+  PCUICWeakening PCUICSubstitution PCUICArities
+  PCUICWcbvEval PCUICSR  PCUICInversion
+  PCUICUnivSubstitution PCUICElimination PCUICCanonicity
+  PCUICUnivSubst PCUICWeakeningEnv PCUICCumulativity.
+
+Require Import Equations.Prop.DepElim.
+
+Local Open Scope string_scope.
+Set Asymmetric Patterns.
+Local Set Keyed Unification.
+
+Import MonadNotation.
+
+Require Import Lia.
+
+Module PA := PCUICAst.
+Module P := PCUICWcbvEval.
+
+Local Existing Instance config.extraction_checker_flags.
+
+(** ** Prelim on arities and proofs *)
+
+Lemma isArity_subst_instance u T :
+  isArity T ->
+  isArity (PCUICUnivSubst.subst_instance_constr u T).
+Proof.
+  induction T; cbn; intros; tauto.
+Qed.
+
+Lemma wf_ext_wk_wf {cf:checker_flags} Σ : wf_ext_wk Σ -> wf Σ.
+Proof. intro H; apply H. Qed.
+
+Hint Resolve wf_ext_wk_wf : core.
+
+Lemma isErasable_subst_instance (Σ : global_env_ext) Γ T univs u :
+  wf_ext_wk Σ ->  wf_local Σ Γ ->
+  wf_local (Σ.1, univs) (PCUICUnivSubst.subst_instance_context u Γ) ->
+  isErasable Σ Γ T ->
+  sub_context_set (monomorphic_udecl Σ.2) (global_ext_context_set (Σ.1, univs)) ->
+  consistent_instance_ext (Σ.1,univs) (Σ.2) u ->
+  isErasable (Σ.1,univs) (PCUICUnivSubst.subst_instance_context u Γ) (PCUICUnivSubst.subst_instance_constr u T).
+Proof.
+  intros. destruct X2 as (? & ? & [ | (? & ? & ?)]).
+  - eapply typing_subst_instance in t; eauto.
+    eexists. split.
+    + eapply t; tas.
+    + left. eapply isArity_subst_instance. eauto.
+  - eapply typing_subst_instance in t; eauto.
+    eexists. split.
+    + eapply t; tas.
+    + right.
+      eapply typing_subst_instance in t0; eauto.
+      eexists. split.
+      * eapply t0; tas.
+      * now eapply is_prop_subst_instance.
+Qed.
+
+(** * Correctness of erasure  *)
+
+Notation "Σ |-p s ▷ t" := (eval Σ s t) (at level 50, s, t at next level) : type_scope.
+Notation "Σ ⊢ s ▷ t" := (Ee.eval Σ s t) (at level 50, s, t at next level) : type_scope.
+
+(** ** Erasure is stable under context conversion *)
+
+Lemma Is_type_conv_context (Σ : global_env_ext) (Γ : context) t (Γ' : context) :
+  wf Σ -> wf_local Σ Γ -> wf_local Σ Γ' ->
+  PCUICContextConversion.conv_context Σ Γ Γ' -> isErasable Σ Γ t -> isErasable Σ Γ' t.
+Proof.
+  intros.
+  destruct X3 as (? & ? & ?). red.
+  exists x. split. eapply PCUICContextConversion.context_conversion. 3:eapply X2. all:eauto.
+  destruct s as [? | [u []]].
+  - left. eauto.
+  - right. exists u. split; eauto. eapply PCUICContextConversion.context_conversion in X2; eauto.
+Qed.
+
+Lemma wf_local_rel_conv:
+  forall Σ : global_env × universes_decl,
+    wf Σ.1 ->
+    forall Γ Γ' : context,
+      PCUICContextConversion.context_relation (PCUICContextConversion.conv_decls Σ) Γ Γ' ->
+      forall Γ0 : context, wf_local Σ Γ' -> wf_local_rel Σ Γ Γ0 -> wf_local_rel Σ Γ' Γ0.
+Proof.
+  intros Σ wfΣ Γ Γ' X1 Γ0 ? w0. induction w0.
+  - econstructor.
+  - econstructor; eauto. cbn in *.
+    destruct t0. exists x. eapply PCUICContextConversion.context_conversion with (Γ ,,, Γ0); eauto.
+    eapply conv_context_app; eauto.
+    eapply typing_wf_local; eauto.
+    eapply PCUICSafeChecker.wf_local_app_inv; eauto.
+  - econstructor; eauto.
+    + cbn in *.
+      destruct t0. exists x. eapply PCUICContextConversion.context_conversion with (Γ ,,, Γ0); eauto.
+      eapply conv_context_app; eauto.
+      eapply typing_wf_local; eauto.
+      eapply PCUICSafeChecker.wf_local_app_inv; eauto.
+    + cbn in *. eapply PCUICContextConversion.context_conversion with (Γ ,,, Γ0); eauto.
+      eapply conv_context_app; eauto.
+      eapply typing_wf_local; eauto.
+      eapply PCUICSafeChecker.wf_local_app_inv; eauto.
+Qed.
+
+Hint Resolve Is_type_conv_context : core.
+
+Lemma erases_context_conversion :
+  env_prop
+  (fun (Σ : PCUICAst.global_env_ext) (Γ : PCUICAst.context) (t T : PCUICAst.term) =>
+      forall Γ' : PCUICAst.context,
+        PCUICContextConversion.conv_context Σ Γ Γ' ->
+        wf_local Σ Γ' ->
+        forall t', erases Σ Γ t t' -> erases Σ Γ' t t')
+  (fun Σ Γ wfΓ => wf_local Σ Γ)
+        .
+Proof.
+  apply typing_ind_env; intros Σ wfΣ Γ wfΓ; intros **; rename_all_hyps; auto.
+  all: match goal with [ H : erases _ _ ?a _ |- ?G ] => tryif is_var a then idtac else inv H end.
+  all: try now (econstructor; eauto).
+  - econstructor. eapply h_forall_Γ'0.
+    econstructor. eauto. now constructor.
+    constructor; auto.
+    exists s1.
+    eapply PCUICContextConversion.context_conversion. 3:eauto. all:eauto.
+  - econstructor. eauto. eapply h_forall_Γ'1.
+    econstructor. eauto. now constructor.
+    constructor; auto. exists s1.
+    eapply PCUICContextConversion.context_conversion with Γ; eauto.
+    eapply PCUICContextConversion.context_conversion with Γ; eauto.
+    eassumption.
+  - econstructor. eauto. eauto.
+    eapply All2_All_left in X3. 2:{ idtac. intros ? ? [[[? e] ?] ?]. exact e. }
+
+    eapply All2_impl. eapply All2_All_mix_left.
+    all: firstorder.
+  - econstructor.
+
+    eapply All2_impl. eapply All2_All_mix_left. eassumption. eassumption.
+    intros. cbn in *.
+    decompose [prod] X2. intuition auto.
+    eapply b0.
+    subst types.
+    eapply conv_context_app; auto. eapply typing_wf_local; eassumption.
+    eapply typing_wf_local in a1. subst types.
+    2:eauto.
+
+    eapply All_local_env_app_inv.
+    eapply All_local_env_app in a1. intuition auto.
+
+    (* clear -wfΣ X2 a2 b4 X1. *)
+    eapply All_local_env_impl; eauto. simpl; intros.
+    destruct T. simpl in *.
+    eapply PCUICContextConversion.context_conversion with (Γ ,,, Γ0); eauto.
+    eapply conv_context_app; auto. eapply typing_wf_local; eauto.
+    eapply typing_wf_local in X3.
+    eapply PCUICSafeChecker.wf_local_app_inv.
+    eauto. eapply wf_local_rel_local in X3.
+    eapply wf_local_rel_app in X3 as []. rewrite app_context_nil_l in w0.
+
+
+    eapply wf_local_rel_conv; eauto.
+    destruct X3. exists x0.
+    eapply PCUICContextConversion.context_conversion with (Γ ,,, Γ0); eauto.
+    eapply conv_context_app; auto. eapply typing_wf_local; eauto.
+
+    eapply typing_wf_local in t0.
+    eapply PCUICSafeChecker.wf_local_app_inv.
+    eauto. eapply wf_local_rel_local in t0.
+    eapply wf_local_rel_app in t0 as []. rewrite app_context_nil_l in w0.
+    eapply wf_local_rel_conv; eauto.
+  - econstructor.
+
+    eapply All2_impl. eapply All2_All_mix_left. eassumption. eassumption.
+    intros. cbn in *.
+    decompose [prod] X2. intuition auto.
+    eapply b0.
+    subst types.
+    eapply conv_context_app; auto. eapply typing_wf_local; eassumption.
+    eapply typing_wf_local in a0. subst types.
+    2:eauto.
+
+    eapply All_local_env_app_inv.
+    eapply All_local_env_app in a0. intuition auto.
+
+    (* clear -wfΣ X2 a2 b4 X1. *)
+    eapply All_local_env_impl; eauto. simpl; intros.
+    destruct T. simpl in *.
+    eapply PCUICContextConversion.context_conversion with (Γ ,,, Γ0); eauto.
+    eapply conv_context_app; auto. eapply typing_wf_local; eauto.
+    eapply typing_wf_local in X3.
+    eapply PCUICSafeChecker.wf_local_app_inv.
+    eauto. eapply wf_local_rel_local in X3.
+    eapply wf_local_rel_app in X3 as []. rewrite app_context_nil_l in w0.
+
+
+    eapply wf_local_rel_conv; eauto.
+    destruct X3. exists x0.
+    eapply PCUICContextConversion.context_conversion with (Γ ,,, Γ0); eauto.
+    eapply conv_context_app; auto. eapply typing_wf_local; eauto.
+
+    eapply typing_wf_local in t0.
+    eapply PCUICSafeChecker.wf_local_app_inv.
+    eauto. eapply wf_local_rel_local in t0.
+    eapply wf_local_rel_app in t0 as []. rewrite app_context_nil_l in w0.
+    eapply wf_local_rel_conv; eauto.
+Qed.
+
+(** ** Erasure is stable under substituting universe constraints  *)
+
+Lemma fix_context_subst_instance:
+  forall (mfix : list (BasicAst.def term)) (u : Instance.t),
+    map (map_decl (PCUICUnivSubst.subst_instance_constr u))
+        (PCUICLiftSubst.fix_context mfix) =
+    PCUICLiftSubst.fix_context
+      (map
+         (map_def (PCUICUnivSubst.subst_instance_constr u)
+                  (PCUICUnivSubst.subst_instance_constr u)) mfix).
+Proof.
+  intros mfix. unfold PCUICLiftSubst.fix_context. intros.
+  rewrite map_rev.
+  rewrite mapi_map.
+  rewrite map_mapi. f_equal. eapply mapi_ext. intros. cbn.
+  unfold map_decl. cbn. unfold vass.
+  rewrite PCUICUnivSubst.lift_subst_instance_constr. reflexivity.
+Qed.
+
+
+
+Lemma erases_subst_instance_constr0
+  : env_prop (fun Σ Γ t T => wf_ext_wk Σ ->
+                           forall t' u univs,
+                             wf_local (Σ.1, univs) (PCUICUnivSubst.subst_instance_context u Γ) ->
+sub_context_set (monomorphic_udecl Σ.2) (global_ext_context_set (Σ.1, univs)) ->
+      consistent_instance_ext (Σ.1,univs) (Σ.2) u ->
+    Σ ;;; Γ |- t ⇝ℇ t' ->
+    (Σ.1,univs) ;;; (PCUICUnivSubst.subst_instance_context u Γ) |- PCUICUnivSubst.subst_instance_constr u t ⇝ℇ t')
+    (fun Σ Γ wfΓ => wf_local Σ Γ).
+Proof.
+  apply typing_ind_env; intros; cbn -[PCUICUnivSubst.subst_instance_constr] in *; auto.
+  all: match goal with [ H : erases _ _ ?a _ |- ?G ] => tryif is_var a then idtac else inv H end.
+  all: try now (econstructor; eauto using isErasable_subst_instance).
+  - cbn. econstructor.
+    eapply H0 in X2; eauto.
+    econstructor. eauto. cbn. econstructor.
+    eapply typing_subst_instance in X0; eauto. apply snd in X0.
+    cbn in X0. refine (X0 _ _ _ _ _); eauto.
+  - cbn. econstructor.
+    eapply H0 in X3; eauto.
+    eapply H1 in X3; eauto. exact X3.
+    econstructor. eauto. cbn. econstructor.
+    eapply typing_subst_instance in X0; eauto. apply snd in X0.
+    cbn in X0. refine (X0 _ _ _ _ _); eauto.
+    cbn. eapply typing_subst_instance in X1; eauto. apply snd in X1.
+    cbn in X1. refine (X1 _ _ _ _ _); eauto.
+  - cbn. econstructor; eauto.
+    eapply All2_map_left.
+    eapply All2_impl. eapply All2_All_mix_left.
+    eapply All2_All_left. exact X3. intros ? ? [[[? e] ?] ?].
+    exact e. exact X6.
+    intros; cbn in *. destruct H. destruct p0. split; eauto.
+  - assert (Hw :  wf_local (Σ.1, univs) (subst_instance_context u (Γ ,,, types))).
+    { (* rewrite subst_instance_context_app. *)
+      assert(All (fun d => isType Σ Γ (dtype d)) mfix).
+      eapply (All_impl X0); firstorder.
+      eapply All_mfix_wf in X5; auto. subst types.
+
+      revert X5. clear - wfΣ wfΓ H2 H3 X2 X3.
+      induction 1.
+      - eauto.
+      - cbn. econstructor; eauto. cbn in *.
+        destruct t0 as (? & ?). eexists.
+        cbn. eapply typing_subst_instance in t0; eauto. apply snd in t0. cbn in t0.
+        rapply t0; eauto.
+      - cbn. econstructor; eauto. cbn in *.
+        destruct t0 as (? & ?). eexists.
+        cbn. eapply typing_subst_instance in t0; eauto. apply snd in t0.
+        rapply t0; eauto.
+        cbn in *. eapply typing_subst_instance in t1; eauto.
+        apply snd in t1. rapply t1. all:eauto.
+    }
+
+    cbn. econstructor; eauto.
+    eapply All2_map_left.
+    eapply All2_impl. eapply All2_All_mix_left. eapply X1.
+    exact X4.
+    intros; cbn in *. destruct X5. destruct p0. destruct p0.
+    destruct p. destruct p. repeat split; eauto.
+    eapply e2 in e1.
+    unfold PCUICUnivSubst.subst_instance_context in *.
+    unfold map_context in *. rewrite map_app in *. subst types. 2:eauto.
+    eapply erases_ctx_ext. eassumption. unfold app_context.
+    f_equal.
+    eapply fix_context_subst_instance. all: eauto.
+
+  - assert (Hw :  wf_local (Σ.1, univs) (subst_instance_context u (Γ ,,, types))).
+  { (* rewrite subst_instance_context_app. *)
+    assert(All (fun d => isType Σ Γ (dtype d)) mfix).
+    eapply (All_impl X0); firstorder.
+    eapply All_mfix_wf in X5; auto. subst types.
+
+    revert X5. clear - wfΣ wfΓ H2 H3 X2 X3.
+    induction 1.
+    - eauto.
+    - cbn. econstructor; eauto. cbn in *.
+      destruct t0 as (? & ?). eexists.
+      cbn. eapply typing_subst_instance in t0; eauto. apply snd in t0. cbn in t0.
+      rapply t0; eauto.
+    - cbn. econstructor; eauto. cbn in *.
+      destruct t0 as (? & ?). eexists.
+      cbn. eapply typing_subst_instance in t0; eauto. apply snd in t0.
+      rapply t0; eauto.
+      cbn in *. eapply typing_subst_instance in t1; eauto.
+      apply snd in t1. rapply t1. all:eauto.
+  }
+
+  cbn. econstructor; eauto.
+  eapply All2_map_left.
+  eapply All2_impl. eapply All2_All_mix_left. eapply X1.
+  exact X4.
+  intros; cbn in *. destruct X5. destruct p0. destruct p0.
+  destruct p. repeat split; eauto.
+  eapply e2 in e1.
+  unfold PCUICUnivSubst.subst_instance_context in *.
+  unfold map_context in *. rewrite map_app in *. subst types. 2:eauto.
+  eapply erases_ctx_ext. eassumption. unfold app_context.
+  f_equal.
+  eapply fix_context_subst_instance. all: eauto.
+
+Qed.
+
+Lemma erases_subst_instance_constr :
+  forall Σ : global_env_ext, wf_ext_wk Σ ->
+  forall Γ, wf_local Σ Γ ->
+  forall t T, Σ ;;; Γ |- t : T ->
+    forall t' u univs,
+  wf_local (Σ.1, univs) (PCUICUnivSubst.subst_instance_context u Γ) ->
+sub_context_set (monomorphic_udecl Σ.2) (global_ext_context_set (Σ.1, univs)) ->      consistent_instance_ext (Σ.1,univs) (Σ.2) u ->
+    Σ ;;; Γ |- t ⇝ℇ t' ->
+    (Σ.1,univs) ;;; (PCUICUnivSubst.subst_instance_context u Γ) |- PCUICUnivSubst.subst_instance_constr u t ⇝ℇ t'.
+Proof.
+  intros Σ X Γ X0 t T X1 t' u univs X2 H H0 H1.
+  unshelve eapply (erases_subst_instance_constr0 Σ _ Γ _ _ _); tea; eauto.
+Qed.
+
+Lemma erases_subst_instance'' Σ φ Γ t T u univs t' :
+  wf_ext_wk (Σ, univs) ->
+  (Σ, univs) ;;; Γ |- t : T ->
+  sub_context_set (monomorphic_udecl univs) (global_context_set Σ) ->
+  consistent_instance_ext (Σ, φ) univs u ->
+  (Σ, univs) ;;; Γ |- t ⇝ℇ t' ->
+  (Σ, φ) ;;; subst_instance_context u Γ
+            |- subst_instance_constr u t ⇝ℇ  t'.
+Proof.
+  intros X X0 X1. intros.
+  eapply (erases_subst_instance_constr (Σ, univs)); tas.
+  eapply typing_wf_local; eassumption. eauto.
+  eapply typing_wf_local.
+  eapply typing_subst_instance''; eauto.
+  etransitivity; tea. apply global_context_set_sub_ext.
+Qed.
+
+Lemma erases_subst_instance_decl Σ Γ t T c decl u t' :
+  wf Σ.1 ->
+  lookup_env Σ.1 c = Some decl ->
+  (Σ.1, universes_decl_of_decl decl) ;;; Γ |- t : T ->
+  consistent_instance_ext Σ (universes_decl_of_decl decl) u ->
+  (Σ.1, universes_decl_of_decl decl) ;;; Γ |- t ⇝ℇ t' ->
+   Σ ;;; subst_instance_context u Γ
+            |- subst_instance_constr u t ⇝ℇ  t'.
+Proof.
+  destruct Σ as [Σ φ]. intros X X0 X1 X2.
+  eapply erases_subst_instance''; tea. split; tas.
+  eapply weaken_lookup_on_global_env'; tea.
+  eapply weaken_lookup_on_global_env''; tea.
+Qed.
+
+(** ** Erasure and applications  *)
+
+Lemma erases_App (Σ : global_env_ext) Γ f L T t :
+  Σ ;;; Γ |- tApp f L : T ->
+  erases Σ Γ (tApp f L) t ->
+  (t = EAst.tBox × squash (isErasable Σ Γ (tApp f L)))
+  \/ exists f' L', t = EAst.tApp f' L' /\
+             erases Σ Γ f f' /\
+             erases Σ Γ L L'.
+Proof.
+  intros. generalize_eqs H.
+  revert f L X.
+  inversion H; intros; try congruence; subst.
+  - inv H4. right. repeat eexists; eauto.
+  - left. split; eauto. econstructor; eauto.
+Qed.
+
+Lemma erases_mkApps (Σ : global_env_ext) Γ f f' L L' :
+  erases Σ Γ f f' ->
+  Forall2 (erases Σ Γ) L L' ->
+  erases Σ Γ (mkApps f L) (EAst.mkApps f' L').
+Proof.
+  intros. revert f f' H; induction H0; cbn; intros; eauto.
+  eapply IHForall2. econstructor. eauto. eauto.
+Qed.
+
+Lemma erases_mkApps_inv (Σ : global_env_ext) Γ f L T t :
+  wf Σ ->
+  Σ ;;; Γ |- mkApps f L : T ->
+  Σ;;; Γ |- mkApps f L ⇝ℇ t ->
+  (exists L1 L2 L2', L = (L1 ++ L2)%list /\
+                squash (isErasable Σ Γ (mkApps f L1)) /\
+                erases Σ Γ (mkApps f L1) EAst.tBox /\
+                Forall2 (erases Σ Γ) L2 L2' /\
+                t = EAst.mkApps EAst.tBox L2'
+  )
+  \/ exists f' L', t = EAst.mkApps f' L' /\
+             erases Σ Γ f f' /\
+             Forall2 (erases Σ Γ) L L'.
+Proof.
+  intros wfΣ. intros. revert f X H ; induction L; cbn in *; intros.
+  - right. exists t, []. cbn. repeat split; eauto.
+  - eapply IHL in H; eauto.
+    destruct H as [ (? & ? & ? & ? & [] & ? & ? & ?) | (? & ? & ? & ? & ?)].
+    + subst. left. exists (a :: x), x0, x1. repeat split; eauto.
+    + subst. eapply PCUICValidity.inversion_mkApps in X as (? & ? & ?); eauto.
+      eapply erases_App in H0 as [ (-> & []) | (? & ? & ? & ? & ?)].
+      * left. exists [a], L, x0. cbn. repeat split. eauto.
+        econstructor; eauto.  eauto.
+      * subst. right. exists x2, (x3 :: x0). repeat split.
+        eauto. econstructor. eauto. eauto.
+      * eauto.
+Qed.
+
+(** ** Global erasure  *)
+
+Lemma lookup_env_erases (Σ : global_env_ext) c decl Σ' :
+  wf Σ ->
+  erases_global Σ Σ' ->
+  lookup_env (fst Σ) c = Some (ConstantDecl decl) ->
+  exists decl', ETyping.lookup_env Σ' c = Some (EAst.ConstantDecl decl') /\
+           erases_constant_body (Σ.1, cst_universes decl)  decl decl'.
+Proof.
+  unfold erases_global. destruct Σ; simpl.
+  intros. induction H; cbn in *.
+  - inv H0.
+  - unfold eq_kername in *; destruct ?.
+    + inv H0.
+      exists cb'. split; eauto. unfold erases_constant_body in *.
+      destruct ?. destruct ?.
+      * destruct decl.
+        eapply (erases_extends (Σ, _)); simpl; eauto. now inv X.
+        2:eexists [_]; simpl; eauto. cbn in *.
+        inv X. cbn in X1.
+        eassumption.
+      * eassumption.
+      * destruct ?; tauto.
+    + edestruct IHerases_global_decls as (decl' & ? & ?).
+      eapply wf_extends.
+      eassumption. now eexists [_]. eauto.
+      destruct decl. cbn in *.
+      exists decl'. split. eauto.
+      unfold erases_constant_body in *. clear H. destruct ?. destruct ?.
+      eapply (@erases_extends (_, _)). 6: eassumption.
+        eapply wf_extends.
+        eassumption. now eexists [_]. eauto.
+        eapply (declared_constant_inv Σ) in H0; eauto.
+        unfold on_constant_decl in H0. rewrite E0 in H0. unfold lift_typing in H0. exact H0.
+        eapply weaken_env_prop_typing. eapply wf_extends. eauto.
+        eexists [_]. reflexivity. eapply wf_extends. eauto. now eexists [_].
+        eauto. now eexists [_].
+      * tauto.
+      * destruct ?; tauto.
+  - unfold eq_kername in *; destruct ?.
+    + inv H0.
+    + edestruct IHerases_global_decls as (decl' & ? & ?).
+      eapply wf_extends.
+      eassumption. now eexists [_]. eauto.
+      exists decl'. split. eauto.
+      unfold erases_constant_body in *. clear H. destruct ?. destruct ?.
+      * eapply (@erases_extends (_,_)). 5: eassumption.
+        eapply wf_extends.
+        eassumption. now eexists [_]. eauto.
+        eapply (declared_constant_inv Σ) in H0; eauto.
+        unfold on_constant_decl in H0. rewrite E0 in H0. unfold lift_typing in H0. eassumption.
+        eapply weaken_env_prop_typing. eapply wf_extends. eauto.
+        eexists [_]. reflexivity. eapply wf_extends. eauto. now eexists [_].
+        eauto. now eexists [_].
+      * tauto.
+      * destruct ?; tauto.
+Qed.
+(** ** The correctness proof  *)
+
+Record extraction_pre (Σ : global_env_ext) : Type
+  := Build_extraction_pre
+  { extr_env_axiom_free' : axiom_free (fst Σ);
+    extr_env_wf' : wf_ext Σ }.
+
+Hint Constructors PCUICWcbvEval.eval erases : core.
+Arguments extr_env_wf' {Σ}.
+Arguments extr_env_axiom_free' {Σ}.
+
+Definition EisConstruct_app :=
+  fun t => match (EAstUtils.decompose_app t).1 with
+        | E.tConstruct _ _ => true
+        | _ => false
+        end.
+
+Lemma fst_decompose_app_rec t l : fst (EAstUtils.decompose_app_rec t l) = fst (EAstUtils.decompose_app t).
+Proof.
+  induction t in l |- *; simpl; auto. rewrite IHt1.
+  unfold decompose_app. simpl. now rewrite (IHt1 [t2]).
+Qed.
+
+Lemma is_construct_erases Σ Γ t t' :
+  Σ;;; Γ |- t ⇝ℇ t' ->
+  negb (isConstruct_app t) -> negb (EisConstruct_app t').
+Proof.
+  induction 1; cbn; try congruence.
+  - unfold isConstruct_app in *. clear IHerases2.
+    cbn. rewrite PCUICInductives.fst_decompose_app_rec.
+    unfold EisConstruct_app in *.
+    cbn. rewrite fst_decompose_app_rec. eassumption.
+Qed.
+
+Lemma is_FixApp_erases Σ Γ t t' :
+  Σ;;; Γ |- t ⇝ℇ t' ->
+  negb (isFixApp t) -> negb (Ee.isFixApp t').
+Proof.
+  induction 1; cbn; try congruence.
+  - unfold isFixApp in *. clear IHerases2.
+    cbn. rewrite PCUICInductives.fst_decompose_app_rec.
+    unfold Ee.isFixApp in *.
+    cbn. rewrite fst_decompose_app_rec. eassumption.
+Qed.
+
+Lemma type_closed_subst {Σ t T} u : wf_ext Σ ->
+  Σ ;;; [] |- t : T ->
+  PCUICLiftSubst.subst1 t 0 u = PCUICCSubst.csubst t 0 u.
+Proof.
+  intros wfΣ tc.
+  apply PCUICClosed.subject_closed in tc; auto.
+  rewrite PCUICCSubst.closed_subst; auto.
+Qed.
+
+Lemma erases_closed Σ Γ  a e : PCUICLiftSubst.closedn #|Γ| a -> Σ ;;; Γ |- a ⇝ℇ e -> closedn #|Γ| e.
+Proof.
+  remember #|Γ| as Γl eqn:Heq.
+  intros cla era.
+  revert Γ e era Heq.
+  pattern Γl, a.
+  match goal with
+  |- ?P Γl a => simpl; eapply (PCUICClosed.term_closedn_list_ind P); auto; clear
+  end; simpl; intros; subst k;
+    match goal with [H:erases _ _ _ _ |- _] => depelim H end; trivial;
+    simpl; try solve [solve_all].
+  - now apply Nat.ltb_lt.
+  - apply andb_and. split; eauto.
+  - apply andb_and; split; eauto.
+  - eapply andb_and; split; eauto.
+    solve_all. destruct y ;  simpl in *; subst.
+    unfold test_snd. simpl; eauto.
+  - epose proof (All2_length _ _ X0).
+    solve_all. destruct y ;  simpl in *; subst.
+    unfold EAst.test_def; simpl; eauto.
+    rewrite <-H. rewrite fix_context_length in b0.
+    eapply b0. eauto. now rewrite app_length, fix_context_length.
+  - epose proof (All2_length _ _ X0).
+    solve_all. destruct y ;  simpl in *; subst.
+    unfold EAst.test_def; simpl; eauto.
+    rewrite <-H. rewrite fix_context_length in b0.
+    eapply b0. eauto. now rewrite app_length, fix_context_length.
+Qed.
+
+Lemma eval_to_mkApps_tBox_inv Σ t argsv :
+  Σ ⊢ t ▷ E.mkApps E.tBox argsv ->
+  argsv = [].
+Proof.
+  intros ev.
+  apply Ee.eval_to_value in ev.
+  now apply value_app_inv in ev.
+Qed.
+
+Transparent PCUICParallelReductionConfluence.construct_cofix_discr.
+
+Lemma erases_correct Σ t T t' v Σ' :
+  extraction_pre Σ ->
+  Σ;;; [] |- t : T ->
+  Σ;;; [] |- t ⇝ℇ t' ->
+  erases_global Σ Σ' ->
+  Σ |-p t ▷ v ->
+  exists v', Σ;;; [] |- v ⇝ℇ v' /\ Σ' ⊢ t' ▷ v'.
+Proof.
+  intros pre Hty He Heg H.
+  revert T Hty t' He.
+  induction H; intros T Hty t' He; inv pre.
+  - assert (Hty' := Hty).
+    assert (eval Σ (PCUICAst.tApp f a) res) by eauto.
+    eapply inversion_App in Hty as (? & ? & ? & ? & ? & ?).
+    inv He.
+
+    + eapply IHeval1 in H4 as (vf' & Hvf' & He_vf'); eauto.
+      eapply IHeval2 in H6 as (vu' & Hvu' & He_vu'); eauto.
+      pose proof (subject_reduction_eval Σ _ _ _ (wf_ext_wf _ extr_env_wf'0) t0 H).
+        eapply inversion_Lambda in X0 as (? & ? & ? & ? & ?).
+        assert (Σ ;;; [] |- a' : t). {
+          eapply subject_reduction_eval; eauto.
+          eapply PCUICConversion.cumul_Prod_inv in c0 as [].
+          econstructor. eassumption. eauto. eapply conv_sym in c0; eauto.
+          now eapply conv_cumul. auto. auto. }
+      assert (eqs := type_closed_subst b extr_env_wf'0  X0).
+      inv Hvf'.
+      * assert (Σ;;; [] |- PCUICLiftSubst.subst1 a' 0 b ⇝ℇ subst1 vu' 0 t').
+        eapply (erases_subst Σ [] [PCUICAst.vass na t] [] b [a'] t'); eauto.
+        econstructor. econstructor. rewrite parsubst_empty. eassumption.
+        rewrite eqs in H2.
+        eapply IHeval3 in H2 as (v' & Hv' & He_v').
+        -- exists v'. split; eauto.
+           econstructor; eauto.
+           rewrite ECSubst.closed_subst; auto.
+           eapply erases_closed in Hvu'; auto.
+           now eapply PCUICClosed.subject_closed in X0.
+        -- rewrite <-eqs. eapply substitution0; eauto.
+      * exists EAst.tBox. split.
+        eapply Is_type_lambda in X1; eauto. destruct X1. econstructor.
+        eapply (is_type_subst Σ [] [PCUICAst.vass na _] [] _ [a']) in X1 ; auto.
+        cbn in X1.
+        eapply Is_type_eval.
+        eauto. eapply H1. rewrite <-eqs. eassumption.
+        all: eauto. econstructor. econstructor. rewrite parsubst_empty.
+        eauto. econstructor. eauto. eauto.
+      * auto.
+    + exists EAst.tBox. split. 2:econstructor; eauto.
+      econstructor.
+      eapply Is_type_eval; eauto.
+    + auto.
+  - assert (Hty' := Hty).
+    assert (Σ |-p tLetIn na b0 t b1 ▷ res) by eauto.
+    eapply inversion_LetIn in Hty' as (? & ? & ? & ? & ? & ?); auto.
+    inv He.
+    + eapply IHeval1 in H6 as (vt1' & Hvt2' & He_vt1'); eauto.
+      assert (Hc : PCUICContextConversion.conv_context Σ ([],, vdef na b0 t) [vdef na b0' t]). {
+        econstructor. econstructor. econstructor.
+        eapply PCUICCumulativity.red_conv.
+        eapply wcbeval_red; eauto. now eapply PCUICClosed.subject_closed in t1. reflexivity.
+      }
+      assert (Σ;;; [vdef na b0' t] |- b1 : x0). {
+        cbn in *. eapply PCUICContextConversion.context_conversion. 3:eauto. all:cbn; eauto.
+        econstructor. all: cbn; eauto. eapply subject_reduction_eval; auto. eauto. eauto.
+      }
+      assert (Σ;;; [] |- PCUICLiftSubst.subst1 b0' 0 b1 ⇝ℇ subst1 vt1' 0 t2'). {
+        eapply (erases_subst Σ [] [PCUICAst.vdef na b0' t] [] b1 [b0'] t2'); eauto.
+        enough (subslet Σ [] [PCUICLiftSubst.subst [] 0 b0'] [vdef na b0' t]).
+        now rewrite parsubst_empty in X1.
+        econstructor. econstructor.
+        rewrite !parsubst_empty.
+        eapply subject_reduction_eval; eauto.
+        eapply erases_context_conversion. 3:eassumption.
+        all: cbn; eauto.
+        econstructor. all: cbn; eauto.
+        eapply subject_reduction_eval; eauto.
+      }
+      unshelve epose proof (subject_reduction_eval _ _ _ _ _ t1 H); eauto.
+      assert (eqs := type_closed_subst b1 extr_env_wf'0 X1).
+      rewrite eqs in H1.
+      eapply IHeval2 in H1 as (vres & Hvres & Hty_vres).
+      2:{ rewrite <-eqs. eapply substitution_let; eauto. }
+      exists vres. split. eauto. econstructor; eauto.
+      enough (ECSubst.csubst vt1' 0 t2'  = t2' {0 := vt1'}) as ->; auto.
+      eapply ECSubst.closed_subst. eapply erases_closed in Hvt2'; auto.
+      eapply eval_closed. eauto. 2:eauto. now eapply PCUICClosed.subject_closed in t1.
+    + exists EAst.tBox. split. 2:econstructor; eauto.
+      econstructor. eapply Is_type_eval; eauto.
+
+  - destruct Σ as (Σ, univs).
+    unfold erases_global in Heg.
+    assert (Σ |-p tConst c u ▷ res) by eauto.
+    eapply inversion_Const in Hty as (? & ? & ? & ? & ?); [|easy].
+    inv He.
+    + assert (isdecl' := isdecl).
+      eapply lookup_env_erases in isdecl; eauto.
+      destruct isdecl as (decl' & ? & ?).
+      unfold erases_constant_body in *. rewrite e in *.
+      destruct ?; try tauto. cbn in *.
+      eapply declared_constant_inj in d; eauto; subst.
+      edestruct IHeval.
+      * cbn in *. pose proof (wf_ext_wf _ extr_env_wf'0). cbn in X0.
+        assert (isdecl'' := isdecl').
+        eapply PCUICWeakeningEnv.declared_constant_inv in isdecl'; eauto.
+        2:eapply PCUICWeakeningEnv.weaken_env_prop_typing.
+        unfold on_constant_decl in isdecl'. rewrite e in isdecl'. red in isdecl'.
+        unfold declared_constant in isdecl''.
+        eapply typing_subst_instance_decl with (Σ0 := (Σ, univs)) (Γ := []); eauto.
+      * pose proof (wf_ext_wf _ extr_env_wf'0). cbn in X0.
+        assert (isdecl'' := isdecl').
+        eapply PCUICWeakeningEnv.declared_constant_inv in isdecl'; eauto.
+        unfold on_constant_decl in isdecl'. rewrite e in isdecl'. cbn in *.
+        2:eapply PCUICWeakeningEnv.weaken_env_prop_typing.
+        eapply erases_subst_instance_decl with (Σ := (Σ, univs)) (Γ := []); eauto.
+      * destruct H2. exists x0. split; eauto. econstructor; eauto.
+    + exists EAst.tBox. split. econstructor.
+      eapply Is_type_eval. 3: eassumption. eauto. eauto. econstructor. eauto.
+
+  - destruct Σ as (Σ, univs).
+    cbn in *.
+    eapply extr_env_axiom_free'0 in isdecl. congruence.
+
+  - assert (Hty' := Hty).
+    assert (Σ |-p tCase (ind, pars) p discr brs ▷ res) by eauto.
+    eapply inversion_Case in Hty' as [u' [args' [mdecl [idecl [ps [pty [btys
+                                    [? [? [? [? [? [_ [? [ht0 [? ?]]]]]]]]]]]]]]]]; auto.
+    assert (Σ ;;; [] |- mkApps (tConstruct ind c u) args :  mkApps (tInd ind u') args').
+    eapply subject_reduction_eval; eauto.
+    eapply PCUICValidity.inversion_mkApps in X0 as (? & ? & ?); eauto.
+    eapply inversion_Construct in t1 as (mdecl' & idecl' & cdecl & ? & ? & ? & ?); auto.
+    assert (d1 := d0).
+    destruct d0.
+    edestruct (declared_inductive_inj H1 d). subst.
+    pose proof (@length_of_btys ind mdecl' idecl' (firstn pars args') u' p).
+    pose proof (length_map_option_out _ _ ht0) as lenbtys. simpl in lenbtys.
+    rewrite H3 in lenbtys.
+
+    inv He.
+    + eapply IHeval1 in H11 as (v' & Hv' & He_v'); eauto.
+      eapply erases_mkApps_inv in Hv' as [(? & ? & ? & ? & [] & ? & ? & ?) | (? & ? & ? & ? & ?)]; eauto.
+      3: eapply subject_reduction_eval; eauto.
+      * subst.
+
+        eapply Is_type_app in X1; auto. destruct X1.
+        2:{ rewrite mkApps_nested. eapply subject_reduction_eval; eauto. }
+        rewrite mkApps_nested in X1.
+
+        eapply tConstruct_no_Type in X1; auto.
+        eapply H10 in X1 as []; eauto. 2: exists []; now destruct Σ.
+
+        destruct (ind_ctors idecl'). cbn in H4. destruct c; inv H2.
+        destruct l; cbn in *; try lia. destruct c as [ | []]; cbn in H2; inv H2.
+
+        destruct btys as [ | ? []]; cbn in H3, lenbtys; try lia. clear H3 lenbtys H4.
+        destruct H7.
+        (* eapply H7 in d1. *) inv a. inv X0.
+        inv X3. inv X4. destruct H7. destruct x3, y; cbn in *; subst.
+        destruct X2. destruct p1; subst; cbn in *.
+        destruct p0 as [narg bty]; simpl in *.
+
+        edestruct (IHeval2) as (? & ? & ?).
+        eapply subject_reduction. eauto. exact Hty.
+        etransitivity.
+        eapply PCUICReduction.red_case_c. eapply wcbeval_red. eauto.
+        now eapply PCUICClosed.subject_closed in t0.
+        eauto.
+        econstructor. econstructor. econstructor.
+
+        all:unfold iota_red in *. all:cbn in *.
+        eapply erases_mkApps. eauto.
+        instantiate (1 := repeat EAst.tBox _).
+        eapply All2_Forall2.
+        eapply All2_impl.
+        eapply All2_All_mix_left. eassumption.
+        2:{ intros. destruct X0. assert (y = EAst.tBox). exact y0. subst. econstructor.
+            now eapply isErasable_Proof. }
+
+        eapply All2_right_triv. 2: now rewrite repeat_length.
+        now eapply All_repeat.
+
+        (* destruct x4; cbn in e2; subst. destruct X2. destruct p0; cbn in e2; subst. cbn in *.  destruct y.  *)
+        exists x3. split; eauto. eapply eval_iota_sing.  2:eauto.
+        pose proof (Ee.eval_to_value _ _ _ He_v').
+        eapply value_app_inv in H4. subst. eassumption.
+
+        eapply wf_ext_wf in extr_env_wf'0.
+        eapply tCase_length_branch_inv in extr_env_wf'0.
+        2:{ eapply subject_reduction. eauto.
+            exact Hty.
+            eapply PCUICReduction.red_case_c. eapply wcbeval_red; eauto.
+            now eapply PCUICClosed.subject_closed in t0. }
+        2: reflexivity.
+
+        enough (#|skipn (ind_npars mdecl') (x0 ++ x1)| = narg) as <- by eauto.
+        rewrite skipn_length. rewrite extr_env_wf'0. lia.
+        rewrite extr_env_wf'0. lia.
+      * subst. unfold iota_red in *.
+        destruct (nth_error brs c) eqn:Hnth.
+        2:{ eapply nth_error_None in Hnth. erewrite All2_length in Hnth. 2:exact a.
+            eapply nth_error_Some_length in H2. cbn in H2. lia. }
+        rewrite <- nth_default_eq in *. unfold nth_default in *.
+        rewrite Hnth in *.
+
+        destruct (All2_nth_error_Some _ _ X0 Hnth) as (? & ? & ? & ?).
+        destruct (All2_nth_error_Some _ _ a Hnth) as (? & ? & ? & ?).
+         destruct p0, x3. cbn in *. subst.
+        edestruct IHeval2 as (? & ? & ?).
+        eapply subject_reduction. eauto. exact Hty.
+        etransitivity.
+        eapply PCUICReduction.red_case_c. eapply wcbeval_red. eauto.
+        now eapply PCUICClosed.subject_closed in t0. eauto.
+
+        etransitivity. eapply trans_red. econstructor.
+        econstructor. unfold iota_red. rewrite <- nth_default_eq. unfold nth_default.
+        rewrite Hnth. econstructor.
+
+        eapply erases_mkApps. eauto.
+        eapply Forall2_skipn. eauto.
+        inv H5.
+        -- exists x3. split; eauto.
+           econstructor. eauto. unfold ETyping.iota_red.
+           rewrite <- nth_default_eq. unfold nth_default. rewrite e1. cbn. eauto.
+        -- eapply Is_type_app in X1 as []; auto.
+           2:{ eapply subject_reduction_eval. 3:eassumption. all: eauto. }
+
+           eapply tConstruct_no_Type in X1; auto.
+           eapply H10 in X1 as []; eauto. 2: exists []; now destruct Σ.
+
+           destruct (ind_ctors idecl'). cbn in H5. destruct c; inv H2.
+           destruct l; cbn in *; try lia. destruct c as [ | []]; cbn in H2; inv H2.
+
+           destruct btys as [ | ? []]; cbn in e4; try discriminate.
+           clear H5. destruct H8.
+            inv a. inv X2. inv X3. inv X0. destruct H9. destruct x0, y; cbn in *; subst.
+           inv X2. destruct p1. subst. destruct p0; cbn in *.
+           destruct X4; subst n1. inv e1. simpl in *. inv Hnth. inv e4. cbn in *.
+
+           edestruct (IHeval2) as (? & ? & ?).
+           eapply subject_reduction. eauto. exact Hty.
+           etransitivity.
+           eapply PCUICReduction.red_case_c. eapply wcbeval_red. eauto.
+           now eapply PCUICClosed.subject_closed in t0; eauto. eauto.
+           econstructor. econstructor.
+           econstructor.
+
+           eapply erases_mkApps. eauto.
+           instantiate (1 := repeat EAst.tBox _).
+           eapply All2_Forall2.
+           eapply All2_impl.
+           eapply All2_All_mix_left. eassumption.
+           2:{ intros. destruct X0. assert (y = EAst.tBox). exact y0. subst. econstructor.
+               now eapply isErasable_Proof. }
+
+           eapply All2_right_triv. 2:now rewrite repeat_length.
+           now eapply All_repeat.
+
+           exists x0. split; eauto.
+           eapply eval_iota_sing.
+           pose proof (Ee.eval_to_value _ _ _ He_v').
+           2:eauto. auto.
+           apply value_app_inv in H8; subst x1.
+           apply He_v'.
+           enough (#|skipn (ind_npars mdecl') args| = n) as <- by eauto.
+
+           eapply wf_ext_wf in extr_env_wf'0.
+           eapply tCase_length_branch_inv in extr_env_wf'0.
+           2:{ eapply subject_reduction. eauto.
+               exact Hty.
+               eapply PCUICReduction.red_case_c. eapply wcbeval_red. eauto.
+               now eapply PCUICClosed.subject_closed in t0. eauto. }
+           2: reflexivity.
+
+           enough (#|skipn (ind_npars mdecl') args| = n) as <- by eauto.
+           rewrite skipn_length. rewrite extr_env_wf'0. lia.
+           rewrite extr_env_wf'0. lia.
+    + exists EAst.tBox. split. econstructor.
+      eapply Is_type_eval; eauto. econstructor; eauto.
+
+  - pose (Hty' := Hty).
+    eapply inversion_Proj in Hty' as (? & ? & ? & [] & ? & ? & ? & ? & ?); [|easy].
+    inv He.
+
+    + eapply IHeval1 in H5 as (vc' & Hvc' & Hty_vc'); eauto.
+      eapply erases_mkApps_inv in Hvc'; eauto.
+      2: eapply subject_reduction_eval; eauto.
+      destruct Hvc' as [ (? & ? & ? & ? & [] & ? & ? & ?) | (? & ? & ? & ? & ?)]; subst.
+      * exists EAst.tBox. split.
+
+        eapply Is_type_app in X as []; eauto. 2:{ rewrite mkApps_nested. eapply subject_reduction_eval; eauto. }
+        rewrite mkApps_nested in X.
+
+        eapply tConstruct_no_Type in X; eauto. eapply H3 in X as [? []]; eauto.
+        2: now destruct d. 2: now exists []; destruct Σ.
+
+        econstructor.
+        eapply Is_type_eval. eauto. eauto.
+        eapply nth_error_all.
+        erewrite nth_error_skipn. reflexivity. eassumption.
+        eapply All_impl. assert (pars = ind_npars x0). destruct d as (? & ? & ?). now rewrite H7. subst.
+        eassumption.
+        eapply isErasable_Proof. eauto.
+
+        eapply eval_proj_box.
+        pose proof (Ee.eval_to_value _ _ _ Hty_vc').
+        eapply value_app_inv in H1. subst. eassumption.
+      * rename H3 into Hinf.
+        eapply Forall2_nth_error_Some in H4 as (? & ? & ?); eauto.
+        assert (Σ ;;; [] |- mkApps (tConstruct i 0 u) args : mkApps (tInd i x) x2).
+        eapply subject_reduction_eval; eauto.
+        eapply PCUICValidity.inversion_mkApps in X as (? & ? & ?); eauto.
+        eapply typing_spine_inv in t2 as []; eauto.
+        eapply IHeval2 in H3 as (? & ? & ?); eauto.
+        inv H2.
+        -- exists x8. split; eauto. econstructor. eauto.
+           rewrite <- nth_default_eq. unfold nth_default. now rewrite H1.
+        -- exists EAst.tBox. split.
+
+
+           eapply Is_type_app in X as []; eauto. 2:{ eapply subject_reduction_eval. 3: eauto. eauto. eauto. }
+
+           eapply tConstruct_no_Type in X. eapply Hinf in X as [? []]; eauto.
+           2: now destruct d. 2: now exists []; destruct Σ.
+
+           econstructor.
+           eapply Is_type_eval. eauto. eauto.
+           eapply nth_error_all.
+           erewrite nth_error_skipn. reflexivity. eassumption.
+           eapply All_impl. assert (pars = ind_npars x0). destruct d as (? & ? & ?). now rewrite H7. subst.
+           eassumption.
+           eapply isErasable_Proof. eauto.
+
+           eapply eval_proj_box.
+           pose proof (Ee.eval_to_value _ _ _ Hty_vc').
+           eapply value_app_inv in H2. subst. eassumption.
+    + exists EAst.tBox. split. econstructor.
+      eapply Is_type_eval. 3: eassumption. eauto. eauto. econstructor. eauto.
+
+  - assert (Hty' := Hty).
+    assert (Hunf := H).
+    assert (Hcon := H1).
+    eapply inversion_App in Hty' as (? & ? & ? & ? & ? & ?); eauto.
+    assert (Ht := t).
+    eapply subject_reduction in t. 2:eauto. 2:eapply wcbeval_red; eauto.
+    2:now eapply PCUICClosed.subject_closed in Ht.
+    assert (HT := t).
+    apply PCUICValidity.inversion_mkApps in HT as (? & ? & ?); auto.
+    assert (Ht1 := t1).
+    apply inversion_Fix in t1 as Hfix; auto.
+    destruct Hfix as (? & ? & ? & ? & ? & ? & ?).
+    rewrite <- closed_unfold_fix_cunfold_eq in e; first last.
+    eapply (PCUICClosed.subject_closed (Γ := [])); eauto.
+    assert (uf := e).
+    unfold unfold_fix in e. rewrite e0 in e. inv e.
+    depelim He; first last.
+
+    + exists EAst.tBox. split; [|now constructor].
+      econstructor.
+      eapply Is_type_eval. eauto. eassumption.
+      eapply Is_type_red. eauto. 2: exact X.
+      cbn.
+      etransitivity.
+      eapply PCUICReduction.red_app.
+      eapply wcbeval_red. eauto. now eapply PCUICClosed.subject_closed in Ht.
+      eauto. eapply wcbeval_red. eauto. now eapply PCUICClosed.subject_closed in t0.
+      eauto.
+      rewrite <- !mkApps_snoc.
+      eapply PCUICReduction.red1_red.
+      eapply red_fix.
+      eauto.
+      unfold is_constructor.
+      rewrite nth_error_snoc; eauto.
+    + eapply IHeval1 in He1 as IH1; eauto.
+      destruct IH1 as (er_stuck_v & er_stuck & ev_stuck).
+      eapply IHeval2 in He2 as IH2; eauto.
+      destruct IH2 as (er_argv & er_arg & ev_arg).
+      eapply erases_mkApps_inv in er_stuck; eauto.
+      destruct er_stuck as [(? & ? & ? & -> & ? & ? & ? & ->)|
+                            (? & ? & -> & ? & ?)].
+      { exists E.tBox.
+        eapply eval_to_mkApps_tBox_inv in ev_stuck as ?; subst.
+        cbn in *.
+        split; [|eauto using Ee.eval].
+        destruct H2.
+        eapply (Is_type_app _ _ _ (x5 ++ [av])) in X as []; eauto; first last.
+        - rewrite mkApps_nested, app_assoc, mkApps_snoc.
+          eapply type_App; eauto.
+          eapply subject_reduction; eauto.
+          eapply wcbeval_red; eauto.
+          eapply PCUICClosed.subject_closed in t0; eauto.
+        - eapply erases_box.
+          eapply Is_type_eval; eauto.
+          eapply Is_type_red; [eauto| |].
+          + rewrite <- mkApps_snoc.
+            eapply PCUICReduction.red1_red.
+            eapply red_fix; [eauto|].
+            unfold is_constructor.
+            now rewrite nth_error_snoc.
+          + rewrite <- app_assoc.
+            now rewrite <- mkApps_nested. }
+
+      inv H2.
+      * assert (Hmfix' := X).
+        eapply All2_nth_error_Some in X as (? & ? & ?); eauto.
+        destruct x3. cbn in *. subst.
+
+        enough (Σ;;; [] ,,, PCUICLiftSubst.subst_context (fix_subst mfix) 0 []
+                |- PCUICLiftSubst.subst (fix_subst mfix) 0 dbody
+                ⇝ℇ subst (ETyping.fix_subst mfix') 0 (Extract.E.dbody x4)).
+        destruct p. destruct p.
+
+        clear e3. rename H into e3.
+        -- cbn in e3. rename x5 into L.
+           eapply (erases_mkApps _ _ _ _ (argsv ++ [av])) in H2; first last.
+           { eapply Forall2_app.
+             - exact H4.
+             - eauto. }
+           rewrite <- mkApps_nested in H2.
+           rewrite EAstUtils.mkApps_app in H2.
+           cbn in *.
+           eapply IHeval3 in H2 as (? & ? & ?); cbn; eauto; first last.
+           { eapply subject_reduction. eauto. exact Hty.
+             etransitivity.
+             eapply PCUICReduction.red_app. eapply wcbeval_red; eauto.
+             now eapply PCUICClosed.subject_closed in Ht.
+             eapply wcbeval_red. eauto. now eapply PCUICClosed.subject_closed in t0.
+             eauto.
+             rewrite <- !mkApps_snoc.
+             eapply PCUICReduction.red1_red.
+             eapply red_fix.
+             eauto.
+             unfold is_constructor.
+             rewrite nth_error_snoc; eauto. }
+
+           exists x3. split. eauto.
+           eapply Ee.eval_fix.
+           ++ eauto.
+           ++ eauto.
+           ++ rewrite <- Ee.closed_unfold_fix_cunfold_eq.
+              { unfold ETyping.unfold_fix. now rewrite e. }
+              eapply eval_closed in e3; eauto.
+              clear -e3 Hmfix'.
+              pose proof (All2_length _ _ Hmfix').
+              eapply PCUICClosed.closedn_mkApps_inv in e3.
+              apply andb_true_iff in e3 as (e3 & _).
+              change (?a = true) with (is_true a) in e3.
+              simpl in e3 |- *. solve_all.
+              rewrite app_context_nil_l in b.
+              eapply erases_closed in b. simpl in b.
+              rewrite <- H.
+              unfold EAst.test_def.
+              simpl in b.
+              rewrite fix_context_length in b.
+              now rewrite Nat.add_0_r.
+              unfold test_def in a. apply andP in a as [_ Hbod].
+              rewrite fix_context_length.
+              now rewrite Nat.add_0_r in Hbod.
+              eauto with pcuic.
+              now eapply PCUICClosed.subject_closed in Ht.
+           ++ apply Forall2_length in H4.
+              congruence.
+           ++ unfold isConstruct_app in *.
+              destruct (decompose_app av) eqn:EE.
+              assert (E2 : fst (decompose_app av) = t3) by now rewrite EE.
+              destruct t3.
+              all:inv i.
+
+              pose proof (decompose_app_rec_inv EE).
+              cbn in H3. subst.
+
+              eapply erases_mkApps_inv in er_arg
+                as [ (? & ? & ? & ? & [] & ? & ? & ?) | (? & ? & ? & ? & ?) ].
+              ** subst.
+                 now apply eval_to_mkApps_tBox_inv in ev_arg as ->.
+              ** subst. inv H5.
+                 +++ destruct x6 using rev_ind; cbn - [EAstUtils.decompose_app]. reflexivity.
+                     unfold is_constructor_app_or_box.
+                     rewrite emkApps_snoc at 1.
+                     now rewrite EAstUtils.decompose_app_mkApps.
+                 +++ now apply eval_to_mkApps_tBox_inv in ev_arg as ->.
+              ** eauto.
+              ** eapply subject_reduction; last first.
+                 eapply wcbeval_red; last first.
+                 eauto.
+                 now eapply PCUICClosed.subject_closed in t0.
+                 eauto.
+                 eauto.
+                 eauto.
+           ++ eauto.
+        -- cbn. destruct p. destruct p.
+           eapply (erases_subst Σ [] (PCUICLiftSubst.fix_context mfix) [] dbody (fix_subst mfix)) in e3; cbn; eauto.
+           ++ eapply subslet_fix_subst. now eapply wf_ext_wf. all: eassumption.
+           ++ eapply nth_error_all in a1; eauto. cbn in a1.
+              eapply a1.
+           ++ eapply All2_from_nth_error.
+              erewrite fix_subst_length, ETyping.fix_subst_length, All2_length; eauto.
+              intros.
+              rewrite fix_subst_nth in H3. 2:{ now rewrite fix_subst_length in H2. }
+              rewrite efix_subst_nth in H5. 2:{ rewrite fix_subst_length in H2.
+                                                erewrite <- All2_length; eauto. }
+              inv H5; inv H3.
+              erewrite All2_length; eauto.
+      * eapply Is_type_app in X as []; tas.
+        -- exists EAst.tBox.
+           split.
+           ++ econstructor.
+              eapply Is_type_eval; eauto.
+              eapply Is_type_red; [eauto| |].
+              ** eapply PCUICReduction.red1_red.
+                 rewrite <- mkApps_snoc.
+                 eapply red_fix; [eauto|].
+                 unfold is_constructor.
+                 now rewrite nth_error_snoc.
+              ** eauto.
+           ++ eapply Ee.eval_box; [|eauto].
+              apply eval_to_mkApps_tBox_inv in ev_stuck as ?; subst.
+              eauto.
+        -- eauto.
+        -- rewrite mkApps_snoc.
+           eapply type_App; eauto.
+           eapply subject_reduction; eauto.
+           eapply wcbeval_red; eauto.
+           eapply PCUICClosed.subject_closed in t0; eauto.
+
+  - apply inversion_App in Hty as Hty'; [|eauto].
+    destruct Hty' as (? & ? & ? & ? & ? & ?).
+
+    eapply subject_reduction in t as typ_stuck_fix; [|eauto|]; first last.
+    { eapply wcbeval_red; [eauto| |eauto].
+      eapply PCUICClosed.subject_closed in t; eauto. }
+
+    eapply erases_App in He as He'; [|eauto].
+    destruct He' as [(-> & [])|(? & ? & -> & ? & ?)].
+    + exists E.tBox.
+      split; [|eauto using Ee.eval].
+      constructor.
+      eapply Is_type_red.
+      * eauto.
+      * eapply PCUICReduction.red_app.
+        -- eapply wcbeval_red; [eauto| |eauto].
+           eapply PCUICClosed.subject_closed in t; eauto.
+        -- eapply wcbeval_red; [eauto| |eauto].
+           eapply PCUICClosed.subject_closed in t0; eauto.
+      * eauto.
+    + eapply subject_reduction in t0 as typ_arg; [|eauto|]; first last.
+      { eapply wcbeval_red; [eauto| |eauto].
+        eapply PCUICClosed.subject_closed in t0; eauto. }
+
+      eapply IHeval1 in H1 as (? & ? & ?); [|eauto].
+      eapply IHeval2 in H2 as (? & ? & ?); [|eauto].
+      eapply erases_mkApps_inv in H1; [|eauto|eauto].
+      destruct H1 as [(? & ? & ? & -> & [] & ? & ? & ->)|(? & ? & -> & ? & ?)].
+      * apply eval_to_mkApps_tBox_inv in H3 as ?; subst.
+        depelim H5.
+        rewrite !app_nil_r in *.
+        cbn in *.
+        exists E.tBox.
+        split; [|eauto using Ee.eval].
+        eapply (Is_type_app _ _ _ [av]) in X as [].
+        -- constructor.
+           apply X.
+        -- eauto.
+        -- eauto.
+        -- cbn.
+           eapply type_App; eauto.
+      * depelim H1.
+        -- exists (E.tApp (E.mkApps (E.tFix mfix' idx) x7) x5).
+           split; [eauto using erases_tApp, erases_mkApps|].
+           unfold cunfold_fix in *.
+           destruct (nth_error _ _) eqn:nth; [|congruence].
+           eapply All2_nth_error_Some in X as (? & ? & ? & ? & ?); [|eauto].
+           eapply Ee.eval_fix_value.
+           ++ eauto.
+           ++ eauto.
+           ++ unfold Ee.cunfold_fix.
+              rewrite e0.
+              reflexivity.
+           ++ eapply Forall2_length in H5.
+              destruct o as [|(<- & ?)]; [left; congruence|right].
+              split; [congruence|].
+              eapply subject_reduction_eval in t; eauto.
+              injection e. intros <- eq.
+              assert (Σ ;;; [] |- mkApps (tFix mfix idx) (argsv ++ [a]) : PCUICLiftSubst.subst1 a 0 x1).
+              { rewrite <-mkApps_nested; simpl. eapply type_App; eauto. }
+              eapply PCUICValidity.inversion_mkApps in X as (fixty & tyfix & sp); auto.
+              eapply inversion_Fix in tyfix as (? & ? & ? & ? & ? & ? & ?); auto.
+              rewrite e4 in nth. injection nth; intros ->.
+              eapply PCUICSpine.typing_spine_strengthen in sp; eauto.
+              eapply wf_fixpoint_spine in sp; eauto.
+              2:{ eapply nth_error_all in a0; eauto. eapply a0. }
+              rewrite eq in sp. rewrite nth_error_app_ge in sp; try lia.
+              rewrite Nat.sub_diag in sp. simpl in sp.
+              destruct sp as [ind [u [indargs [tya ck]]]].
+              eapply wf_ext_wf in extr_env_wf'0.
+              pose proof (eval_ind_canonical Σ _ _ _ _ extr_env_axiom_free'0 tya _ H0).
+              revert H1 H6.
+              unfold negb, isConstruct_app, PCUICParallelReductionConfluence.construct_cofix_discr, PCUICInductives.head.
+              destruct (decompose_app av) as [hd tl] eqn:da. simpl.
+              destruct hd; try congruence. intros _ _.
+              eapply subject_reduction_eval in tya; eauto.
+              eapply decompose_app_inv in da. subst av.
+              eapply typing_cofix_coind in tya; auto.
+              pose proof (check_recursivity_kind_inj Σ ck tya).
+              now discriminate.
+
+        -- exists E.tBox.
+           apply eval_to_mkApps_tBox_inv in H3 as ?; subst.
+           split; [|eauto using Ee.eval].
+           eapply Is_type_app in X as [].
+           ++ constructor.
+              rewrite <- mkApps_snoc.
+              exact X.
+           ++ eauto.
+           ++ eauto.
+           ++ rewrite mkApps_snoc.
+              eapply type_App; eauto.
+
+  - destruct ip.
+    assert (Hty' := Hty).
+    eapply inversion_Case in Hty' as [u' [args' [mdecl [idecl [ps [pty [btys
+                                   [? [? [? [? [? [_ [? [ht0 [? ?]]]]]]]]]]]]]]]];
+    eauto.
+    eapply PCUICValidity.inversion_mkApps in t0 as (? & ? & ?); eauto.
+    eapply inversion_CoFix in t0 as (? & ? & ? &?); eauto.
+    todo "erasure cofix"%string.
+
+  - assert (Hty' := Hty).
+    eapply inversion_Proj in Hty' as (? & ? & ? & [] & ? & ? & ? & ? & ?).
+    eapply PCUICValidity.inversion_mkApps in t0 as (? & ? & ?); eauto.
+    eapply inversion_CoFix in t0 as (? & ? & ? &?); eauto.
+    todo "erasure cofix". auto.
+  - pose (Hty' := Hty).
+    eapply inversion_App in Hty' as (? & ? & ? & ? & ? & ?); eauto.
+    inv He.
+    + assert (t' := t). eapply IHeval1 in t as (? & ? & ?); eauto.
+      eapply IHeval2 in t0 as (? & ? & ?); eauto.
+      destruct (EAstUtils.isBox x2) eqn:E.
+      * destruct x2; inv E. exists EAst.tBox. split. 2: econstructor; eauto.
+        pose proof (Is_type_app Σ [] f'[a']).
+        inversion H1.
+        edestruct H7; eauto. cbn. eapply subject_reduction. eauto.
+        exact Hty. eapply PCUICReduction.red_app.
+        eapply PCUICClosed.subject_closed in t'; auto.
+        eapply wcbeval_red; eauto.
+        eapply inversion_App in Hty as [na [A [B [Hf [Ha _]]]]]; auto.
+        eapply PCUICClosed.subject_closed in Ha; auto.
+        eapply wcbeval_red; eauto.
+      * exists (E.tApp x2 x3).
+        split. 2:{ eapply Ee.eval_app_cong; eauto.
+                   eapply ssrbool.negbT.
+                   repeat eapply orb_false_intro.
+                   - destruct x2; try reflexivity.
+                     inv H1. inv i.
+                   - destruct x2 eqn:Ex; try reflexivity.
+                     + cbn. inv H1. cbn in *.
+                       eapply ssrbool.negbTE, is_FixApp_erases.
+                       econstructor; eauto.
+                       now rewrite orb_false_r in i.
+                     + cbn in *.
+                       inv H1. inv i.
+                   - eauto. }
+        econstructor; eauto.
+    + exists EAst.tBox. split. 2: now econstructor.
+      econstructor.
+      eapply inversion_App in Hty as [na [A [B [Hf [Ha _]]]]]; auto.
+      eapply Is_type_red. 3:eauto. eauto.
+      eapply PCUICReduction.red_app.
+      eapply PCUICClosed.subject_closed in Hf; auto.
+      eapply wcbeval_red; eauto.
+      eapply PCUICClosed.subject_closed in Ha; auto.
+      eapply wcbeval_red; eauto.
+
+  - destruct t; try easy.
+    + inv He. eexists. split; eauto. now econstructor.
+    + inv He. eexists. split; eauto. now econstructor.
+    + inv He.
+      * eexists. split; eauto. now econstructor.
+      * eexists. split. 2: now econstructor.
+        econstructor; eauto.
+    + inv He.
+      * eexists. split. 2: now econstructor.
+        econstructor; eauto.
+    + inv He.
+      * eexists. split. 2: now econstructor.
+        econstructor; eauto.
+      * eexists. split. 2: now econstructor.
+        eauto.
+    + inv He.
+      * eexists. split; eauto. now econstructor.
+      * eexists. split. 2: now econstructor.
+        econstructor; eauto.
+    + inv He.
+      * eexists. split; eauto. now econstructor.
+      * eexists. split. 2: now econstructor.
+        econstructor; eauto.
+Qed.
+
+Print Assumptions erases_correct.
